lib/zoo_parabs/waiters.ml
@@ -10,7 +10,7 @@ let create sz =
 
 let notify t i =
   let waiter = Array.unsafe_get t.waiters i in
-  Waiter.notify_strong waiter
+  Waiter.notify waiter |> ignore
 
 let rec notify_one t =
   match Mpmc_queue_1.pop t.queue with
