theories/examples/vertex_fibonacci.v
@@ -1,13 +1,14 @@
 From zoo Require Import
   prelude.
 From zoo.iris.base_logic Require Import
-  lib.fupd.
+  lib.fupd
+  lib.saved_prop.
 From zoo.language Require Import
   notations.
 From zoo.diaframe Require Import
   diaframe.
 From zoo_std Require Import
-  mpsc_flag.
+  ivar_3.
 From zoo_parabs Require Import
   pool
   vertex.
@@ -18,18 +19,20 @@ From zoo Require Import
   options.
 
 Implicit Types r : location.
-Implicit Types ctx vtx : val.
+Implicit Types v ctx vtx : val.
 
 Class VertexFibonacciG Σ `{zoo_G : !ZooG Σ} :=
   { #[local] vertex_fibonacci_G_pool_G :: PoolG Σ
   ; #[local] vertex_fibonacci_G_vertex_G :: VertexG Σ
-  ; #[local] vertex_fibonacci_G_mpsc_flag_G :: MpscFlagG Σ
+  ; #[local] vertex_fibonacci_G_ivar_G :: Ivar3G Σ gname
+  ; #[local] vertex_fibonacci_G_saved_prop_G :: SavedPropG Σ
   }.
 
 Definition vertex_fibonacci_Σ := #[
   pool_Σ ;
   vertex_Σ ;
-  mpsc_flag_Σ
+  ivar_3_Σ gname ;
+  saved_prop_Σ
 ].
 #[global] Instance subG_vertex_fibonacci_Σ Σ `{zoo_G : !ZooG Σ} :
   subG vertex_fibonacci_Σ Σ →
@@ -142,16 +145,21 @@ Section vertex_fibonacci_G.
       wp_apply+ (vertex_release𑁒spec with "[$Hctx $Hvtx1_inv $Hvtx1_model Hr]") as "Hctx".
       { iApply (vertex_fibonacci_main₀𑁒spec with "Hvtx1_inv Hr"). }
 
-      wp_apply+ (mpsc_flag_create𑁒spec
-        (r ↦ᵣ #(fibonacci n))
-      with "[//]") as (flag) "(#Hflag_inv & Hflag_consumer)".
+      wp_apply+ (ivar_3_create𑁒spec
+        (λ _, r ↦ᵣ #(fibonacci n))%I
+        (λ _, True)%I
+        ( λ _ waiter _,
+          ∀ ctx v,
+          WP waiter ctx v {{ itype_unit }}
+        )%I
+      with "[//]") as (ivar) "(#Hivar_inv & Hivar_producer & Hivar_consumer)".
 
       wp_apply+ (vertex_create'𑁒spec
         True
         True
       with "[//]") as (vtx2 iter2) "(#Hvtx2_inv & Hvtx2_model & _)".
       wp_apply+ (vertex_precede𑁒spec with "[$Hvtx2_model]") as "(Hvtx2_model & #Hvtx1_predecessor)". 1: iFrame "#".
-      wp_apply+ (vertex_release𑁒spec' with "[$Hctx $Hvtx2_model Hvtx1_output]") as "Hctx".
+      wp_apply+ (vertex_release𑁒spec' with "[$Hctx $Hvtx2_model Hvtx1_output Hivar_producer]") as "Hctx".
       { iFrame "#". iIntros "{%} %pool %ctx %scope Hctx #Hvtx2_ready".
 
         wp_pures credits:"H£".
@@ -160,19 +168,12 @@ Section vertex_fibonacci_G.
         iDestruct (vertex_predecessor_finished with "Hvtx1_predecessor Hvtx2_ready") as "#Hvtx1_finished".
         iMod (vertex_inv_finished_output' with "H£ Hvtx1_inv Hvtx1_finished Hvtx1_output") as "Hr".
 
-        wp_apply+ (mpsc_flag_set𑁒spec with "[$Hflag_inv $Hr]").
+        wp_apply+ (ivar_3_notify𑁒spec True with "[$Hivar_inv $Hivar_producer $Hr]"). 1: iSteps.
         iSteps.
       }
 
-      wp_apply+ (pool_wait_until𑁒spec
-        (mpsc_flag_consumer flag)
-        (r ↦ᵣ #(fibonacci n))
-      with "[$Hctx Hflag_consumer]").
-      { iStep 3 as "Hflag_consumer".
-        wp_apply+ (mpsc_flag_get𑁒spec with "[$Hflag_inv $Hflag_consumer]").
-        iSteps.
-      }
-
+      wp_apply+ (pool_wait_ivar𑁒spec with "[$Hctx $Hivar_inv]") as "(H£ & $ & (%v & #Hivar_result))". 1: iSteps.
+      iMod (ivar_3_inv_result_consumer' with "H£ Hivar_inv Hivar_result Hivar_consumer") as "(Hr & _)".
       iSteps.
     }
 
